src/impl/TLS13.Impl.ConnectionState.LocalHandshake.fst
@@ -3121,7 +3121,7 @@ fn install_server_handshake_write_traffic_keys_from_material
               };
             }))
 {
-  let aead_key_len = read_negotiated_aead_key_len c;
+  let aead_alg = read_negotiated_aead_alg c;
   let install = Ghost.hide {
     CS.install_epoch = CS.TrafficHandshake;
     CS.install_direction = CS.TrafficWrite;
@@ -3149,7 +3149,7 @@ fn install_server_handshake_write_traffic_keys_from_material
   store_traffic_key_material
     c.handshake.keys.server_handshake_traffic
     traffic_secret_src
-    aead_key_len
+    aead_alg
     traffic_key_src
     traffic_iv_src
     #material;
@@ -3157,7 +3157,7 @@ fn install_server_handshake_write_traffic_keys_from_material
     c.handshake.keys
     (installed_traffic_keys_for_role_state st0 (Ghost.reveal role_install)).CS.cs_model.CS.model_handshake.CS.hs_keys);
 
-  Rec.install_handshake_keys_runtime c.records.write traffic_key_src aead_key_len (Ghost.hide (Ghost.reveal material).CS.traffic_key) traffic_iv_src;
+  Rec.install_handshake_keys_runtime c.records.write traffic_key_src aead_alg (Ghost.hide (Ghost.reveal material).CS.traffic_key) traffic_iv_src;
   assert (pure ((Ghost.reveal install).CS.install_epoch == CS.TrafficHandshake));
   assert (pure ((Ghost.reveal install).CS.install_direction == CS.TrafficWrite));
   assert (pure ((Ghost.reveal install).CS.install_material == Ghost.reveal material));
@@ -3348,7 +3348,7 @@ fn install_client_handshake_read_traffic_keys_from_material
               };
             }))
 {
-  let aead_key_len = read_negotiated_aead_key_len c;
+  let aead_alg = read_negotiated_aead_alg c;
   let install = Ghost.hide {
     CS.install_epoch = CS.TrafficHandshake;
     CS.install_direction = CS.TrafficRead;
@@ -3376,7 +3376,7 @@ fn install_client_handshake_read_traffic_keys_from_material
   store_traffic_key_material
     c.handshake.keys.client_handshake_traffic
     traffic_secret_src
-    aead_key_len
+    aead_alg
     traffic_key_src
     traffic_iv_src
     #material;
@@ -3384,7 +3384,7 @@ fn install_client_handshake_read_traffic_keys_from_material
     c.handshake.keys
     (installed_traffic_keys_for_role_state st0 (Ghost.reveal role_install)).CS.cs_model.CS.model_handshake.CS.hs_keys);
 
-  Rec.install_handshake_keys_runtime c.records.read traffic_key_src aead_key_len (Ghost.hide (Ghost.reveal material).CS.traffic_key) traffic_iv_src;
+  Rec.install_handshake_keys_runtime c.records.read traffic_key_src aead_alg (Ghost.hide (Ghost.reveal material).CS.traffic_key) traffic_iv_src;
   assert (pure ((Ghost.reveal install).CS.install_epoch == CS.TrafficHandshake));
   assert (pure ((Ghost.reveal install).CS.install_direction == CS.TrafficRead));
   assert (pure ((Ghost.reveal install).CS.install_material == Ghost.reveal material));
@@ -3575,7 +3575,7 @@ fn install_server_application_write_traffic_keys_from_material
               };
             }))
 {
-  let aead_key_len = read_negotiated_aead_key_len c;
+  let aead_alg = read_negotiated_aead_alg c;
   let install = Ghost.hide {
     CS.install_epoch = CS.TrafficApplication;
     CS.install_direction = CS.TrafficWrite;
@@ -3603,7 +3603,7 @@ fn install_server_application_write_traffic_keys_from_material
   store_traffic_key_material
     c.handshake.keys.server_application_traffic
     traffic_secret_src
-    aead_key_len
+    aead_alg
     traffic_key_src
     traffic_iv_src
     #material;
@@ -3611,7 +3611,7 @@ fn install_server_application_write_traffic_keys_from_material
     c.handshake.keys
     (installed_traffic_keys_for_role_state st0 (Ghost.reveal role_install)).CS.cs_model.CS.model_handshake.CS.hs_keys);
 
-  Rec.install_application_keys_runtime c.records.write traffic_key_src aead_key_len (Ghost.hide (Ghost.reveal material).CS.traffic_key) traffic_iv_src;
+  Rec.install_application_keys_runtime c.records.write traffic_key_src aead_alg (Ghost.hide (Ghost.reveal material).CS.traffic_key) traffic_iv_src;
   assert (pure ((Ghost.reveal install).CS.install_epoch == CS.TrafficApplication));
   assert (pure ((Ghost.reveal install).CS.install_direction == CS.TrafficWrite));
   assert (pure ((Ghost.reveal install).CS.install_material == Ghost.reveal material));
@@ -3803,7 +3803,7 @@ fn install_client_application_read_traffic_keys_from_material
               };
             }))
 {
-  let aead_key_len = read_negotiated_aead_key_len c;
+  let aead_alg = read_negotiated_aead_alg c;
   let install = Ghost.hide {
     CS.install_epoch = CS.TrafficApplication;
     CS.install_direction = CS.TrafficRead;
@@ -3831,7 +3831,7 @@ fn install_client_application_read_traffic_keys_from_material
   store_traffic_key_material
     c.handshake.keys.client_application_traffic
     traffic_secret_src
-    aead_key_len
+    aead_alg
     traffic_key_src
     traffic_iv_src
     #material;
@@ -3839,7 +3839,7 @@ fn install_client_application_read_traffic_keys_from_material
     c.handshake.keys
     (installed_traffic_keys_for_role_state st0 (Ghost.reveal role_install)).CS.cs_model.CS.model_handshake.CS.hs_keys);
 
-  Rec.install_application_keys_runtime c.records.read traffic_key_src aead_key_len (Ghost.hide (Ghost.reveal material).CS.traffic_key) traffic_iv_src;
+  Rec.install_application_keys_runtime c.records.read traffic_key_src aead_alg (Ghost.hide (Ghost.reveal material).CS.traffic_key) traffic_iv_src;
   assert (pure ((Ghost.reveal install).CS.install_epoch == CS.TrafficApplication));
   assert (pure ((Ghost.reveal install).CS.install_direction == CS.TrafficRead));
   assert (pure ((Ghost.reveal install).CS.install_material == Ghost.reveal material));
@@ -4015,7 +4015,7 @@ fn derive_and_install_server_application_write_traffic_keys
                 };
               }))
 {
-  let aead_key_len = read_negotiated_aead_key_len c;
+  let aead_alg = read_negotiated_aead_alg c;
   unfold (connection_exactly c st0);
   unfold (connection_model_exactly c st0.CS.cs_model);
   unfold (control_exactly c.control st0.CS.cs_model.CS.model_control st0.CS.cs_model.CS.model_failure);
@@ -4086,14 +4086,14 @@ fn derive_and_install_server_application_write_traffic_keys
       (Tr.hash st0.CS.cs_model.CS.model_handshake.CS.hs_transcript)));
 
   let mut traffic_key_out = [| 0uy; 32sz |];
-  KS.derive_traffic_key traffic_secret_out aead_key_len traffic_key_out;
+  KS.derive_traffic_key traffic_secret_out aead_alg traffic_key_out;
   let mut traffic_iv_out = [| 0uy; 12sz |];
   KS.derive_traffic_iv traffic_secret_out traffic_iv_out;
   with traffic_key_bytes. assert (ArrPts.pts_to traffic_key_out traffic_key_bytes);
   with traffic_iv_bytes. assert (ArrPts.pts_to traffic_iv_out traffic_iv_bytes);
 
   let traffic_secret = Ghost.hide traffic_secret_bytes;
-  let material = Ghost.hide (CS.traffic_key_material_for_secret (TLS13.Crypto.Spec.aead_alg_of_key_len (SZ.v aead_key_len)) (Ghost.reveal traffic_secret));
+  let material = Ghost.hide (CS.traffic_key_material_for_secret (aead_alg) (Ghost.reveal traffic_secret));
   assert (pure ((Ghost.reveal material).CS.traffic_secret == traffic_secret_bytes));
   assert (pure (Seq.equal traffic_key_bytes (TLS13.Crypto.Spec.pad_key_32 (Ghost.reveal material).CS.traffic_key)));
   assert (pure ((Ghost.reveal material).CS.traffic_iv == traffic_iv_bytes));
@@ -4184,7 +4184,7 @@ fn derive_and_install_client_application_read_traffic_keys
                 };
               }))
 {
-  let aead_key_len = read_negotiated_aead_key_len c;
+  let aead_alg = read_negotiated_aead_alg c;
   unfold (connection_exactly c st0);
   unfold (connection_model_exactly c st0.CS.cs_model);
   unfold (control_exactly c.control st0.CS.cs_model.CS.model_control st0.CS.cs_model.CS.model_failure);
@@ -4255,14 +4255,14 @@ fn derive_and_install_client_application_read_traffic_keys
       (Tr.hash st0.CS.cs_model.CS.model_handshake.CS.hs_transcript)));
 
   let mut traffic_key_out = [| 0uy; 32sz |];
-  KS.derive_traffic_key traffic_secret_out aead_key_len traffic_key_out;
+  KS.derive_traffic_key traffic_secret_out aead_alg traffic_key_out;
   let mut traffic_iv_out = [| 0uy; 12sz |];
   KS.derive_traffic_iv traffic_secret_out traffic_iv_out;
   with traffic_key_bytes. assert (ArrPts.pts_to traffic_key_out traffic_key_bytes);
   with traffic_iv_bytes. assert (ArrPts.pts_to traffic_iv_out traffic_iv_bytes);
 
   let traffic_secret = Ghost.hide traffic_secret_bytes;
-  let material = Ghost.hide (CS.traffic_key_material_for_secret (TLS13.Crypto.Spec.aead_alg_of_key_len (SZ.v aead_key_len)) (Ghost.reveal traffic_secret));
+  let material = Ghost.hide (CS.traffic_key_material_for_secret (aead_alg) (Ghost.reveal traffic_secret));
   assert (pure ((Ghost.reveal material).CS.traffic_secret == traffic_secret_bytes));
   assert (pure (Seq.equal traffic_key_bytes (TLS13.Crypto.Spec.pad_key_32 (Ghost.reveal material).CS.traffic_key)));
   assert (pure ((Ghost.reveal material).CS.traffic_iv == traffic_iv_bytes));
@@ -4353,7 +4353,7 @@ fn derive_and_install_server_handshake_write_traffic_keys
                 };
               }))
 {
-  let aead_key_len = read_negotiated_aead_key_len c;
+  let aead_alg = read_negotiated_aead_alg c;
   unfold (connection_exactly c st0);
   unfold (connection_model_exactly c st0.CS.cs_model);
   unfold (control_exactly c.control st0.CS.cs_model.CS.model_control st0.CS.cs_model.CS.model_failure);
@@ -4424,14 +4424,14 @@ fn derive_and_install_server_handshake_write_traffic_keys
       (Tr.hash st0.CS.cs_model.CS.model_handshake.CS.hs_transcript)));
 
   let mut traffic_key_out = [| 0uy; 32sz |];
-  KS.derive_traffic_key traffic_secret_out aead_key_len traffic_key_out;
+  KS.derive_traffic_key traffic_secret_out aead_alg traffic_key_out;
   let mut traffic_iv_out = [| 0uy; 12sz |];
   KS.derive_traffic_iv traffic_secret_out traffic_iv_out;
   with traffic_key_bytes. assert (ArrPts.pts_to traffic_key_out traffic_key_bytes);
   with traffic_iv_bytes. assert (ArrPts.pts_to traffic_iv_out traffic_iv_bytes);
 
   let traffic_secret = Ghost.hide traffic_secret_bytes;
-  let material = Ghost.hide (CS.traffic_key_material_for_secret (TLS13.Crypto.Spec.aead_alg_of_key_len (SZ.v aead_key_len)) (Ghost.reveal traffic_secret));
+  let material = Ghost.hide (CS.traffic_key_material_for_secret (aead_alg) (Ghost.reveal traffic_secret));
   assert (pure ((Ghost.reveal material).CS.traffic_secret == traffic_secret_bytes));
   assert (pure (Seq.equal traffic_key_bytes (TLS13.Crypto.Spec.pad_key_32 (Ghost.reveal material).CS.traffic_key)));
   assert (pure ((Ghost.reveal material).CS.traffic_iv == traffic_iv_bytes));
@@ -4522,7 +4522,7 @@ fn derive_and_install_client_handshake_read_traffic_keys
                 };
               }))
 {
-  let aead_key_len = read_negotiated_aead_key_len c;
+  let aead_alg = read_negotiated_aead_alg c;
   unfold (connection_exactly c st0);
   unfold (connection_model_exactly c st0.CS.cs_model);
   unfold (control_exactly c.control st0.CS.cs_model.CS.model_control st0.CS.cs_model.CS.model_failure);
@@ -4593,14 +4593,14 @@ fn derive_and_install_client_handshake_read_traffic_keys
       (Tr.hash st0.CS.cs_model.CS.model_handshake.CS.hs_transcript)));
 
   let mut traffic_key_out = [| 0uy; 32sz |];
-  KS.derive_traffic_key traffic_secret_out aead_key_len traffic_key_out;
+  KS.derive_traffic_key traffic_secret_out aead_alg traffic_key_out;
   let mut traffic_iv_out = [| 0uy; 12sz |];
   KS.derive_traffic_iv traffic_secret_out traffic_iv_out;
   with traffic_key_bytes. assert (ArrPts.pts_to traffic_key_out traffic_key_bytes);
   with traffic_iv_bytes. assert (ArrPts.pts_to traffic_iv_out traffic_iv_bytes);
 
   let traffic_secret = Ghost.hide traffic_secret_bytes;
-  let material = Ghost.hide (CS.traffic_key_material_for_secret (TLS13.Crypto.Spec.aead_alg_of_key_len (SZ.v aead_key_len)) (Ghost.reveal traffic_secret));
+  let material = Ghost.hide (CS.traffic_key_material_for_secret (aead_alg) (Ghost.reveal traffic_secret));
   assert (pure ((Ghost.reveal material).CS.traffic_secret == traffic_secret_bytes));
   assert (pure (Seq.equal traffic_key_bytes (TLS13.Crypto.Spec.pad_key_32 (Ghost.reveal material).CS.traffic_key)));
   assert (pure ((Ghost.reveal material).CS.traffic_iv == traffic_iv_bytes));
@@ -5205,7 +5205,7 @@ fn try_install_client_handshake_traffic_keys
            else
              connection_exactly c st0)
 {
-  let aead_key_len = read_negotiated_aead_key_len c;
+  let aead_alg = read_negotiated_aead_alg c;
   let ready = can_install_handshake_traffic_keys c;
   if ready {
     unfold (connection_exactly c st0);
@@ -5281,14 +5281,14 @@ fn try_install_client_handshake_traffic_keys
         (Tr.hash st0.CS.cs_model.CS.model_handshake.CS.hs_transcript)));
 
     let mut traffic_key_out = [| 0uy; 32sz |];
-    KS.derive_traffic_key traffic_secret_out aead_key_len traffic_key_out;
+    KS.derive_traffic_key traffic_secret_out aead_alg traffic_key_out;
     let mut traffic_iv_out = [| 0uy; 12sz |];
     KS.derive_traffic_iv traffic_secret_out traffic_iv_out;
     with traffic_key_bytes. assert (ArrPts.pts_to traffic_key_out traffic_key_bytes);
     with traffic_iv_bytes. assert (ArrPts.pts_to traffic_iv_out traffic_iv_bytes);
 
     let traffic_secret = Ghost.hide traffic_secret_bytes;
-    let material = Ghost.hide (CS.traffic_key_material_for_secret (TLS13.Crypto.Spec.aead_alg_of_key_len (SZ.v aead_key_len)) (Ghost.reveal traffic_secret));
+    let material = Ghost.hide (CS.traffic_key_material_for_secret (aead_alg) (Ghost.reveal traffic_secret));
     assert (pure ((Ghost.reveal material).CS.traffic_secret == traffic_secret_bytes));
     assert (pure (Seq.equal traffic_key_bytes (TLS13.Crypto.Spec.pad_key_32 (Ghost.reveal material).CS.traffic_key)));
     assert (pure ((Ghost.reveal material).CS.traffic_iv == traffic_iv_bytes));
@@ -5308,7 +5308,7 @@ fn try_install_client_handshake_traffic_keys
     store_traffic_key_material
       c.handshake.keys.client_handshake_traffic
       traffic_secret_out
-      aead_key_len
+      aead_alg
       traffic_key_out
       traffic_iv_out
       #material;
@@ -5319,7 +5319,7 @@ fn try_install_client_handshake_traffic_keys
       c.handshake.keys
       (installed_traffic_keys_state st0 (Ghost.reveal install)).CS.cs_model.CS.model_handshake.CS.hs_keys);
 
-    Rec.install_handshake_keys_runtime c.records.write traffic_key_out aead_key_len (Ghost.hide (Ghost.reveal material).CS.traffic_key) traffic_iv_out;
+    Rec.install_handshake_keys_runtime c.records.write traffic_key_out aead_alg (Ghost.hide (Ghost.reveal material).CS.traffic_key) traffic_iv_out;
     assert (pure ((Ghost.reveal install).CS.install_epoch == CS.TrafficHandshake));
     assert (pure ((Ghost.reveal install).CS.install_direction == CS.TrafficWrite));
     assert (pure ((Ghost.reveal install).CS.install_material == Ghost.reveal material));
@@ -5494,7 +5494,7 @@ fn try_install_server_handshake_traffic_keys
            else
              connection_exactly c st0)
 {
-  let aead_key_len = read_negotiated_aead_key_len c;
+  let aead_alg = read_negotiated_aead_alg c;
   let ready = can_install_handshake_traffic_keys c;
   if ready {
     unfold (connection_exactly c st0);
@@ -5570,14 +5570,14 @@ fn try_install_server_handshake_traffic_keys
         (Tr.hash st0.CS.cs_model.CS.model_handshake.CS.hs_transcript)));
 
     let mut traffic_key_out = [| 0uy; 32sz |];
-    KS.derive_traffic_key traffic_secret_out aead_key_len traffic_key_out;
+    KS.derive_traffic_key traffic_secret_out aead_alg traffic_key_out;
     let mut traffic_iv_out = [| 0uy; 12sz |];
     KS.derive_traffic_iv traffic_secret_out traffic_iv_out;
     with traffic_key_bytes. assert (ArrPts.pts_to traffic_key_out traffic_key_bytes);
     with traffic_iv_bytes. assert (ArrPts.pts_to traffic_iv_out traffic_iv_bytes);
 
     let traffic_secret = Ghost.hide traffic_secret_bytes;
-    let material = Ghost.hide (CS.traffic_key_material_for_secret (TLS13.Crypto.Spec.aead_alg_of_key_len (SZ.v aead_key_len)) (Ghost.reveal traffic_secret));
+    let material = Ghost.hide (CS.traffic_key_material_for_secret (aead_alg) (Ghost.reveal traffic_secret));
     assert (pure ((Ghost.reveal material).CS.traffic_secret == traffic_secret_bytes));
     assert (pure (Seq.equal traffic_key_bytes (TLS13.Crypto.Spec.pad_key_32 (Ghost.reveal material).CS.traffic_key)));
     assert (pure ((Ghost.reveal material).CS.traffic_iv == traffic_iv_bytes));
@@ -5597,7 +5597,7 @@ fn try_install_server_handshake_traffic_keys
     store_traffic_key_material
       c.handshake.keys.server_handshake_traffic
       traffic_secret_out
-      aead_key_len
+      aead_alg
       traffic_key_out
       traffic_iv_out
       #material;
@@ -5608,7 +5608,7 @@ fn try_install_server_handshake_traffic_keys
       c.handshake.keys
       (installed_traffic_keys_state st0 (Ghost.reveal install)).CS.cs_model.CS.model_handshake.CS.hs_keys);
 
-    Rec.install_handshake_keys_runtime c.records.read traffic_key_out aead_key_len (Ghost.hide (Ghost.reveal material).CS.traffic_key) traffic_iv_out;
+    Rec.install_handshake_keys_runtime c.records.read traffic_key_out aead_alg (Ghost.hide (Ghost.reveal material).CS.traffic_key) traffic_iv_out;
     assert (pure ((Ghost.reveal install).CS.install_epoch == CS.TrafficHandshake));
     assert (pure ((Ghost.reveal install).CS.install_direction == CS.TrafficRead));
     assert (pure ((Ghost.reveal install).CS.install_material == Ghost.reveal material));
@@ -5782,7 +5782,7 @@ fn try_install_client_application_traffic_keys
            else
              connection_exactly c st0)
 {
-  let aead_key_len = read_negotiated_aead_key_len c;
+  let aead_alg = read_negotiated_aead_alg c;
   let ready = can_install_application_traffic_keys c;
   if ready {
     unfold (connection_exactly c st0);
@@ -5858,14 +5858,14 @@ fn try_install_client_application_traffic_keys
         (Tr.hash st0.CS.cs_model.CS.model_handshake.CS.hs_transcript)));
 
     let mut traffic_key_out = [| 0uy; 32sz |];
-    KS.derive_traffic_key traffic_secret_out aead_key_len traffic_key_out;
+    KS.derive_traffic_key traffic_secret_out aead_alg traffic_key_out;
     let mut traffic_iv_out = [| 0uy; 12sz |];
     KS.derive_traffic_iv traffic_secret_out traffic_iv_out;
     with traffic_key_bytes. assert (ArrPts.pts_to traffic_key_out traffic_key_bytes);
     with traffic_iv_bytes. assert (ArrPts.pts_to traffic_iv_out traffic_iv_bytes);
 
     let traffic_secret = Ghost.hide traffic_secret_bytes;
-    let material = Ghost.hide (CS.traffic_key_material_for_secret (TLS13.Crypto.Spec.aead_alg_of_key_len (SZ.v aead_key_len)) (Ghost.reveal traffic_secret));
+    let material = Ghost.hide (CS.traffic_key_material_for_secret (aead_alg) (Ghost.reveal traffic_secret));
     assert (pure ((Ghost.reveal material).CS.traffic_secret == traffic_secret_bytes));
     assert (pure (Seq.equal traffic_key_bytes (TLS13.Crypto.Spec.pad_key_32 (Ghost.reveal material).CS.traffic_key)));
     assert (pure ((Ghost.reveal material).CS.traffic_iv == traffic_iv_bytes));
@@ -5885,7 +5885,7 @@ fn try_install_client_application_traffic_keys
     store_traffic_key_material
       c.handshake.keys.client_application_traffic
       traffic_secret_out
-      aead_key_len
+      aead_alg
       traffic_key_out
       traffic_iv_out
       #material;
@@ -6059,7 +6059,7 @@ fn try_install_server_application_traffic_keys
            else
              connection_exactly c st0)
 {
-  let aead_key_len = read_negotiated_aead_key_len c;
+  let aead_alg = read_negotiated_aead_alg c;
   let ready = can_install_application_traffic_keys c;
   if ready {
     unfold (connection_exactly c st0);
@@ -6135,14 +6135,14 @@ fn try_install_server_application_traffic_keys
         (Tr.hash st0.CS.cs_model.CS.model_handshake.CS.hs_transcript)));
 
     let mut traffic_key_out = [| 0uy; 32sz |];
-    KS.derive_traffic_key traffic_secret_out aead_key_len traffic_key_out;
+    KS.derive_traffic_key traffic_secret_out aead_alg traffic_key_out;
     let mut traffic_iv_out = [| 0uy; 12sz |];
     KS.derive_traffic_iv traffic_secret_out traffic_iv_out;
     with traffic_key_bytes. assert (ArrPts.pts_to traffic_key_out traffic_key_bytes);
     with traffic_iv_bytes. assert (ArrPts.pts_to traffic_iv_out traffic_iv_bytes);
 
     let traffic_secret = Ghost.hide traffic_secret_bytes;
-    let material = Ghost.hide (CS.traffic_key_material_for_secret (TLS13.Crypto.Spec.aead_alg_of_key_len (SZ.v aead_key_len)) (Ghost.reveal traffic_secret));
+    let material = Ghost.hide (CS.traffic_key_material_for_secret (aead_alg) (Ghost.reveal traffic_secret));
     assert (pure ((Ghost.reveal material).CS.traffic_secret == traffic_secret_bytes));
     assert (pure (Seq.equal traffic_key_bytes (TLS13.Crypto.Spec.pad_key_32 (Ghost.reveal material).CS.traffic_key)));
     assert (pure ((Ghost.reveal material).CS.traffic_iv == traffic_iv_bytes));
@@ -6162,7 +6162,7 @@ fn try_install_server_application_traffic_keys
     store_traffic_key_material
       c.handshake.keys.server_application_traffic
       traffic_secret_out
-      aead_key_len
+      aead_alg
       traffic_key_out
       traffic_iv_out
       #material;
@@ -6173,7 +6173,7 @@ fn try_install_server_application_traffic_keys
       c.handshake.keys
       (installed_traffic_keys_state st0 (Ghost.reveal install)).CS.cs_model.CS.model_handshake.CS.hs_keys);
 
-    Rec.install_application_keys_runtime c.records.read traffic_key_out aead_key_len (Ghost.hide (Ghost.reveal material).CS.traffic_key) traffic_iv_out;
+    Rec.install_application_keys_runtime c.records.read traffic_key_out aead_alg (Ghost.hide (Ghost.reveal material).CS.traffic_key) traffic_iv_out;
     assert (pure ((Ghost.reveal install).CS.install_epoch == CS.TrafficApplication));
     assert (pure ((Ghost.reveal install).CS.install_direction == CS.TrafficRead));
     assert (pure ((Ghost.reveal install).CS.install_material == Ghost.reveal material));
